Converted to structured proofs

Cancelation.thy
@@ -23,18 +23,18 @@ These were helpfully provided by Andreas Lochbihler.
 *}
 
 theorem lconfluent_confluent:
-  "[| wfP (R^--1); !!a b c. R a b ==> R a c ==> \<exists>d. R^** b d \<and> R^** c d  |] ==> confluent R"
+  "\<lbrakk> wfP (R^--1); \<And>a b c. R a b \<Longrightarrow> R a c \<Longrightarrow> \<exists>d. R^** b d \<and> R^** c d  \<rbrakk> \<Longrightarrow> confluent R"
 by(auto simp add: diamond_def commute_def square_def intro: newman)
 
 lemma confluentD:
-  "[| confluent R; R^** a b; R^** a c  |] ==> \<exists>d. R^** b d \<and> R^** c d"
+  "\<lbrakk> confluent R; R^** a b; R^** a c  \<rbrakk> \<Longrightarrow> \<exists>d. R^** b d \<and> R^** c d"
 by(auto simp add: commute_def diamond_def square_def)
 
-lemma tranclp_DomainP: "R^++ a b ==> DomainP R a"
+lemma tranclp_DomainP: "R^++ a b \<Longrightarrow> DomainP R a"
 by(auto elim: converse_tranclpE)
 
 lemma confluent_unique_normal_form:
-  "[| confluent R; R^** a b; R^** a c; ~ DomainP R b; ~ DomainP R c  |] ==> b = c"
+  "\<lbrakk> confluent R; R^** a b; R^** a c; \<not> DomainP R b; \<not> DomainP R c  \<rbrakk> \<Longrightarrow> b = c"
 apply(drule confluentD[of R a b c], assumption+)
 apply clarify
 apply(drule rtranclpD[where a=b])
@@ -55,28 +55,23 @@ These type aliases encode the notion of a ``generator or its inverse''
 (* Too bad I cannot use antiquotations _before_ the definition, it would make
 the text easier to read. *)
 
-definition canceling :: "'a g_i => 'a g_i => bool"
- where "canceling a b = ((snd a = snd b) \<and> (fst a ~= fst b))"
+definition canceling :: "'a g_i \<Rightarrow> 'a g_i \<Rightarrow> bool"
+ where "canceling a b = ((snd a = snd b) \<and> (fst a \<noteq> fst b))"
 
 text {*
 A generators cancels with its inverse, either way.
 *}
 
 subsubsection {* Simple results about canceling *}
-lemma cancel_cancel: "[| canceling a b ; canceling b c  |] ==> a = c"
-apply (simp add:canceling_def)
-apply(rule prod_eqI)
-apply auto
-done
 
-lemma cancel_sym: "canceling a b ==> canceling b a"
-apply (simp add:canceling_def)
-done
+lemma cancel_cancel: "\<lbrakk> canceling a b; canceling b c \<rbrakk> \<Longrightarrow> a = c"
+by (auto intro: prod_eqI simp add:canceling_def)
 
-lemma cancel_sym_neg: "~canceling a b ==> ~canceling b a"
-apply (rule classical)
-apply (simp add:canceling_def)
-done
+lemma cancel_sym: "canceling a b \<Longrightarrow> canceling b a"
+by (simp add:canceling_def)
+
+lemma cancel_sym_neg: "\<not>canceling a b \<Longrightarrow> \<not>canceling b a"
+by (rule classical, simp add:canceling_def)
 
 subsection {* Definition of the @{term "cancels_to"} relation *}
 
@@ -85,23 +80,29 @@ First, we define the function that removes the @{term i}th and @{text "(i+1)"}st
 element from a word of generators, together with basic properties.
 *}
 
-definition cancel_at :: "nat => 'a word_g_i => 'a word_g_i"
+definition cancel_at :: "nat \<Rightarrow> 'a word_g_i \<Rightarrow> 'a word_g_i"
 where "cancel_at i l = take i l @ drop (2+i) l"
 
-lemma cancel_at_length[simp]: "[| 1+i < length l  |] ==> length (cancel_at i l) = length l - 2"
-apply(auto simp add: cancel_at_def)
-done
+lemma cancel_at_length[simp]:
+  "1+i < length l \<Longrightarrow> length (cancel_at i l) = length l - 2"
+by(auto simp add: cancel_at_def)
 
-lemma cancel_at_nth1[simp]: "[| n < i; 1+i < length l  |] ==> (cancel_at i l) ! n = l !n"
-apply(auto simp add: cancel_at_def nth_append)
-done
+lemma cancel_at_nth1[simp]:
+  "\<lbrakk> n < i; 1+i < length l  \<rbrakk> \<Longrightarrow> (cancel_at i l) ! n = l ! n"
+by(auto simp add: cancel_at_def nth_append)
 
-lemma cancel_at_nth2[simp]: "[| n \<ge> i; n < length l - 2  |] ==> (cancel_at i l) ! n = l ! (n + 2)"
-apply(auto simp add: cancel_at_def nth_append nth_via_drop)
-apply(subgoal_tac "i = min (length l) i")
-prefer 2
-apply auto
-done
+
+lemma cancel_at_nth2[simp]:
+  assumes "n \<ge> i" and "n < length l - 2"
+  shows "(cancel_at i l) ! n = l ! (n + 2)"
+proof-
+  from `n \<ge> i` and `n < length l - 2`
+  have "i = min (length l) i"
+    by auto
+  with `n \<ge> i` and `n < length l - 2`
+  show "(cancel_at i l) ! n = l ! (n + 2)" 
+    by(auto simp add: cancel_at_def nth_append nth_via_drop)
+qed
 
 text {*
 Then we can define the relation @{term "cancels_to_1_at i a b"} which specifies
@@ -115,19 +116,22 @@ transitive hull.
 A word is @{text "canceled"} if it can not be canceled any futher.
 *}
 
-definition cancels_to_1_at ::  "nat => 'a word_g_i => 'a word_g_i => bool"
+definition cancels_to_1_at ::  "nat \<Rightarrow> 'a word_g_i \<Rightarrow> 'a word_g_i \<Rightarrow> bool"
 where  "cancels_to_1_at i l1 l2 = (0\<le>i \<and> (1+i) < length l1
                               \<and> canceling (l1 ! i) (l1 ! (1+i))
                               \<and> (l2 = cancel_at i l1))"
 
-definition cancels_to_1 :: "'a word_g_i => 'a word_g_i => bool"
+definition cancels_to_1 :: "'a word_g_i \<Rightarrow> 'a word_g_i \<Rightarrow> bool"
 where "cancels_to_1 l1 l2 = (\<exists>i. cancels_to_1_at i l1 l2)"
 
-definition cancels_to  :: "'a word_g_i => 'a word_g_i => bool"
+definition cancels_to  :: "'a word_g_i \<Rightarrow> 'a word_g_i \<Rightarrow> bool"
 where "cancels_to = cancels_to_1^**"
 
-definition canceled :: "'a word_g_i => bool"
- where "canceled l = (~ DomainP cancels_to_1 l)"
+lemma cancels_to_trans: "\<lbrakk> cancels_to a b; cancels_to b c \<rbrakk> \<Longrightarrow> cancels_to a c"
+by (auto simp add:cancels_to_def)
+
+definition canceled :: "'a word_g_i \<Rightarrow> bool"
+ where "canceled l = (\<not> DomainP cancels_to_1 l)"
 
 (*
 lemma "cancels_to_1 [(True,(1::nat)),(False,1)] []"
@@ -143,141 +147,226 @@ One of two steps to show that we have a normal form is the following lemma,
 quaranteeing that by canceling, we always end up at a fully canceled word.
 *}
 
+(*
+I turned this proof into the next, structured proof. But is this really an improvement?
 lemma canceling_terminates: "wfP (cancels_to_1^--1)"
 apply(simp add:wfP_def)
 apply (rule_tac r = "measure size" in wf_subset)
 apply(auto simp add: cancels_to_1_def cancel_at_def cancels_to_1_at_def)
 done
-
-lemma cancels_to_1E: "[| cancels_to_1 l1 l2 ;
-  !! i. [| cancels_to_1_at i l1 l2   |]
-   ==> P  |] ==> P"
-apply (auto  simp add:cancels_to_1_def)
-done
+*)
+lemma canceling_terminates: "wfP (cancels_to_1^--1)"
+proof-
+  have "wf (measure length)" by auto
+  have "{(x, y). cancels_to_1 y x} \<subseteq> measure length"
+    by (auto simp add: cancels_to_1_def cancel_at_def cancels_to_1_at_def)
+  with `wf (measure length)`
+  have "wf {(x, y). cancels_to_1 y x}"
+    by(rule_tac r = "measure size" in wf_subset)
+  thus ?thesis by (simp add:wfP_def)
+qed
 
 text {*
-The next two lemmas preper for the proof of confluence. It does not matter in
+The next two lemmas prepare for the proof of confluence. It does not matter in
 which order we cancel, we can obtain the same result.
 *}
 
-lemma canceling_neighbor: "[| cancels_to_1_at i l a; cancels_to_1_at (Suc i) l b  |] ==> a = b"
-apply(auto simp add: cancel_at_def cancels_to_1_at_def)
-apply(subgoal_tac "l ! i = l ! Suc (Suc i)")
-prefer 2
-apply(erule cancel_cancel)
-apply assumption
-apply(thin_tac "canceling ?x ?y")
-apply(thin_tac "canceling ?x ?y")
-apply(case_tac "drop (Suc (Suc i)) l")
-apply auto[1]
-apply(auto simp add: take_Suc_conv_app_nth)
-apply(subgoal_tac "(a,b)=l!i")
-apply auto[1]
-apply(simp only:nth_via_drop)
-apply(subgoal_tac "list = tl (drop (Suc (Suc i)) l)")
-apply(auto simp add:drop_tl drop_Suc)
-done
+lemma canceling_neighbor:
+  assumes "cancels_to_1_at i l a" and "cancels_to_1_at (Suc i) l b"
+  shows "a = b"
+proof-
+  from `cancels_to_1_at i l a`
+    have "canceling (l ! i) (l ! Suc i)" and "i < length l"
+    by (auto simp add: cancels_to_1_at_def)
+  
+  from `cancels_to_1_at (Suc i) l b`
+    have "canceling (l ! Suc i) (l ! Suc (Suc i))" and "Suc (Suc i) < length l"
+    by (auto simp add: cancels_to_1_at_def)
 
-lemma canceling_indep: "[| cancels_to_1_at i l a; cancels_to_1_at j l b ; j > Suc i |] ==> \<exists> c. cancels_to_1_at (j - 2) a c \<and> cancels_to_1_at i b c"
-apply(auto simp add:  cancels_to_1_at_def)[1]
+  from `canceling (l ! i) (l ! Suc i)` and `canceling (l ! Suc i) (l ! Suc (Suc i))`
+    have "l ! i = l ! Suc (Suc i)" by (rule cancel_cancel)
 
-apply(auto simp add:cancel_at_def)
-apply(subgoal_tac "Suc (Suc (j - 2)) = j")
-prefer 2
-apply auto[1]
-apply auto[1]
+  from `cancels_to_1_at (Suc i) l b`
+    have "b = take (Suc i) l @ drop (Suc (Suc (Suc i))) l"
+    by (simp add: cancels_to_1_at_def cancel_at_def)
+  moreover from `i < length l`
+    have "\<dots> = take i l @ [l ! i] @ drop (Suc (Suc (Suc i))) l"
+    by(auto simp add: take_Suc_conv_app_nth)
+  moreover from `l ! i = l ! Suc (Suc i)`
+    have "\<dots> = take i l @ [l ! Suc (Suc i)] @ drop (Suc (Suc (Suc i))) l"
+    by simp
+  moreover from `Suc (Suc i) < length l`
+    have "\<dots> = take i l @ drop (Suc (Suc i)) l"
+    by (simp add: drop_Suc_conv_tl)
+  moreover from `cancels_to_1_at i l a` have
+    "\<dots> = a"
+    by (simp add: cancels_to_1_at_def cancel_at_def)
+  ultimately show "a = b"
+    by (simp )
+qed
 
-apply(thin_tac "canceling ?x ?y")
-apply(thin_tac "canceling ?x ?y")
+lemma canceling_indep:
+  assumes "cancels_to_1_at i l a" and "cancels_to_1_at j l b" and "j > Suc i"
+  shows "\<exists> c. cancels_to_1_at (j - 2) a c \<and> cancels_to_1_at i b c"
+proof-
+  from `cancels_to_1_at i l a`
+    have "Suc i < length l"
+     and "canceling (l ! i) (l ! Suc i)"
+     and "a = cancel_at i l"
+     and "length a = length l - 2"
+     and "min (length l) i = i"
+    by (auto simp add:cancels_to_1_at_def)
+  from `cancels_to_1_at j l b`
+    have "Suc j < length l"
+     and "canceling (l ! j) (l ! Suc j)"
+     and "b = cancel_at j l"
+     and "length b = length l - 2"
+    by (auto simp add:cancels_to_1_at_def)
 
-apply(subgoal_tac "min i j = i")
-prefer 2
-apply auto[1]
-apply simp
+  let ?c = "cancel_at (j - 2) a"
+  have "cancels_to_1_at (j - 2) a ?c \<and> cancels_to_1_at i b ?c"
+  proof
+    from `j > Suc i`
+      have "Suc (Suc (j - 2)) = j"
+       and "Suc (Suc (Suc j - 2)) = Suc j"
+      by auto
+    with `min (length l) i = i` and `j > Suc i` and `Suc j < length l`
+    have "(l ! j) = (cancel_at i l ! (j - 2))"
+     and "(l ! (Suc j)) = (cancel_at i l ! Suc (j - 2))"
+     by(auto simp add:cancel_at_def simp add:nth_append)
 
-apply(subgoal_tac "min (length l) i = i")
-prefer 2
-apply auto[1]
-apply simp
+    with `cancels_to_1_at i l a`
+     and `cancels_to_1_at j l b`
+    have "canceling (a ! (j - 2)) (a ! Suc (j - 2))"
+      by(auto simp add:cancels_to_1_at_def)
 
-apply(subgoal_tac "min (j - 2) i = i")
-prefer 2
-apply auto[1]
-apply simp
+    with `j > Suc i` and `Suc j < length l` and `length a = length l - 2`
+    show "cancels_to_1_at (j - 2) a ?c" by (auto simp add: cancels_to_1_at_def)
+  next
+    from `length b = length l - 2` and `j > Suc i` and `Suc j < length l`
+      have "Suc i < length b" by auto
 
-apply(thin_tac "min ?x ?y = ?z")
-apply(thin_tac "min ?x ?y = ?z")
-apply(thin_tac "min ?x ?y = ?z")
+    moreover from `b = cancel_at j l` and `j > Suc i` and `Suc i < length l`
+      have "(b ! i) = (l ! i)" and "(b ! Suc i) = (l ! Suc i)"
+      by (auto simp add:cancel_at_def nth_append)
+    with `canceling (l ! i) (l ! Suc i)`
+      have "canceling (b ! i) (b ! Suc i)" by simp
 
-apply(subgoal_tac "(Suc (Suc (j + i - 2))) = j+i")
-prefer 2
-apply auto[1]
-apply (simp add:drop_take)
-done
+    moreover from `j > Suc i` and `Suc j < length l`
+      have "min i j = i"
+       and "min (j - 2) i = i"
+       and "min (length l) j = j"
+       and "min (length l) i = i"
+       and "Suc (Suc (j - 2)) = j"
+      by auto
+    with `a = cancel_at i l` and `b = cancel_at j l` and `Suc (Suc (j - 2)) = j`
+      have "cancel_at (j - 2) a = cancel_at i b"
+      by (auto simp add:cancel_at_def take_drop)
+
+    ultimately show "cancels_to_1_at i b (cancel_at (j - 2) a)"
+      by (auto simp add:cancels_to_1_at_def)
+  qed
+  thus ?thesis by(rule exI)
+qed (* This takes very long in i3p. Why? I just showed everything? Can I speed it up? *)
 
 text {* This is the confluence lemma *}
 
 lemma lconf: "confluent cancels_to_1"
-apply(rule lconfluent_confluent)
-apply(rule canceling_terminates)
-apply(simp add: cancels_to_1_def)
-apply(erule exE)
-apply(erule exE)
-apply(rename_tac a b c i j)
+proof(rule lconfluent_confluent)
+  show "wfP cancels_to_1\<inverse>\<inverse>" by (rule canceling_terminates)
+next
+  fix a b c
+  assume "cancels_to_1 a b"
+  then obtain i where "cancels_to_1_at i a b" by -(simp add: cancels_to_1_def, erule exE)
+  assume "cancels_to_1 a c"
+  then obtain j where "cancels_to_1_at j a c" by -(simp add: cancels_to_1_def, erule exE)
 
-apply(case_tac "j=i")
-apply(simp add: cancels_to_1_at_def)
-apply(rule_tac x="b" in exI)
-apply auto[1]
-
-apply(case_tac "j=Suc i")
-apply clarsimp
-apply(rule_tac x="b" in exI)
-apply(subgoal_tac "b=c")
-prefer 2
-apply(erule canceling_neighbor)
-apply assumption
-apply auto[1]
-
-apply(case_tac "i=Suc j")
-apply clarsimp
-apply(rule_tac x="c" in exI)
-apply(subgoal_tac "c=b")
-prefer 2
-apply(erule canceling_neighbor)
-apply assumption
-apply auto[1]
-
-apply(subgoal_tac "\<exists>d. cancels_to_1 b d \<and> cancels_to_1 c d")
-apply auto[1]
-apply(simp add:cancels_to_1_def)
-
-apply(case_tac "i<j")
-apply(subgoal_tac "\<exists>d. cancels_to_1_at (j - 2) b d \<and> cancels_to_1_at i c d")
-apply auto[1]
-apply(erule canceling_indep)
-apply auto[2]
-
-apply(subgoal_tac "\<exists>d. cancels_to_1_at (i - 2) c d \<and> cancels_to_1_at j b d")
-apply auto[1]
-apply(erule canceling_indep)
-apply auto[2]
-done
+  show "\<exists>d. cancels_to_1\<^sup>*\<^sup>* b d \<and> cancels_to_1\<^sup>*\<^sup>* c d"
+  proof (cases "i=j")
+    assume "i=j"
+    from `cancels_to_1_at i a b`
+      have "b = cancel_at i a" by (simp add:cancels_to_1_at_def)
+    moreover from `i=j`
+      have "\<dots> = cancel_at j a" by (clarify)
+    moreover from `cancels_to_1_at j a c`
+      have "\<dots> = c" by (simp add:cancels_to_1_at_def)
+    ultimately have "b = c" by (simp)
+    hence "cancels_to_1\<^sup>*\<^sup>* b b"
+      and "cancels_to_1\<^sup>*\<^sup>* c b" by auto
+    thus "\<exists>d. cancels_to_1\<^sup>*\<^sup>* b d \<and> cancels_to_1\<^sup>*\<^sup>* c d" by blast
+  next 
+    assume "i \<noteq> j"
+    show ?thesis
+    proof (cases "j = Suc i")
+      assume "j = Suc i"
+        with `cancels_to_1_at i a b` and `cancels_to_1_at j a c`
+        have "b = c" by (auto elim: canceling_neighbor)
+      hence "cancels_to_1\<^sup>*\<^sup>* b b"
+        and "cancels_to_1\<^sup>*\<^sup>* c b" by auto
+      thus "\<exists>d. cancels_to_1\<^sup>*\<^sup>* b d \<and> cancels_to_1\<^sup>*\<^sup>* c d" by blast
+    next
+      assume "j \<noteq> Suc i"
+      show ?thesis
+      proof (cases "i = Suc j")
+        assume "i = Suc j"
+          with `cancels_to_1_at i a b` and `cancels_to_1_at j a c`
+          have "c = b" by (auto elim: canceling_neighbor)
+        hence "cancels_to_1\<^sup>*\<^sup>* b b"
+          and "cancels_to_1\<^sup>*\<^sup>* c b" by auto
+        thus "\<exists>d. cancels_to_1\<^sup>*\<^sup>* b d \<and> cancels_to_1\<^sup>*\<^sup>* c d" by blast
+      next
+        assume "i \<noteq> Suc j"
+        show ?thesis
+        proof (cases "i < j")
+          assume "i < j"
+            with `j \<noteq> Suc i` have "Suc i < j" by auto
+          with `cancels_to_1_at i a b` and `cancels_to_1_at j a c`
+            have "\<exists>d. cancels_to_1_at (j - 2) b d \<and> cancels_to_1_at i c d" by (auto elim: canceling_indep)
+          then obtain d where "cancels_to_1_at (j - 2) b d \<and> cancels_to_1_at i c d" by (erule exE)
+          hence "cancels_to_1 b d \<and> cancels_to_1 c d" by (auto simp add:cancels_to_1_def)
+          thus "\<exists>d. cancels_to_1\<^sup>*\<^sup>* b d \<and> cancels_to_1\<^sup>*\<^sup>* c d" by (auto)
+        next
+          assume "\<not> i < j"
+            with `j \<noteq> Suc i` and `i \<noteq> j` and `i \<noteq> Suc j` have "Suc j < i" by auto
+          with `cancels_to_1_at i a b` and `cancels_to_1_at j a c`
+            have "\<exists>d. cancels_to_1_at (i - 2) c d \<and> cancels_to_1_at j b d" by (auto elim: canceling_indep)
+          then obtain d where "cancels_to_1_at (i - 2) c d \<and> cancels_to_1_at j b d" by (erule exE)
+          hence "cancels_to_1 b d \<and> cancels_to_1 c d" by (auto simp add:cancels_to_1_def)
+          thus "\<exists>d. cancels_to_1\<^sup>*\<^sup>* b d \<and> cancels_to_1\<^sup>*\<^sup>* c d" by (auto)
+        qed
+      qed
+    qed
+  qed
+qed
 
 text {*
 And finally, we show that there exists a unique normal form for each word.
 *}
 
-lemma inv_rtrcl: "R^**^--1 = R^--1^**"
+lemma inv_rtrcl: "R^**^--1 = R^--1^**" (* Did I overlook this in the standard libs? *)
 apply (auto simp add:expand_fun_eq intro: dest:rtranclp_converseD intro:rtranclp_converseI)
 done
 
-lemma norm_form_uniq: "[| cancels_to a b; cancels_to a c; canceled b; canceled c  |] ==> b = c"
-apply(simp add: cancels_to_def canceled_def)
-apply(rule_tac R="cancels_to_1" and a="a" in confluent_unique_normal_form)
-apply(rule lconf)
-apply auto
-done
+lemma norm_form_uniq:
+  assumes "cancels_to a b"
+      and "cancels_to a c"
+      and "canceled b"
+      and "canceled c"
+  shows "b = c"
+proof-
+  have "confluent cancels_to_1" by (rule lconf)
+  moreover 
+  from `cancels_to a b` have "cancels_to_1^** a b" by (simp add: cancels_to_def)
+  moreover
+  from `cancels_to a c` have "cancels_to_1^** a c" by (simp add: cancels_to_def)
+  moreover
+  from `canceled b` have "\<not> DomainP cancels_to_1 b" by (simp add: canceled_def)
+  moreover
+  from `canceled c` have "\<not> DomainP cancels_to_1 c" by (simp add: canceled_def)
+  ultimately
+  show "b = c"
+    by (rule confluent_unique_normal_form)
+qed
 
 subsubsection {* Some properties on cancelation *}
 
@@ -285,56 +374,62 @@ text {*
 Distributivity rules of cancelation and @{text append}.
 *}
 
-lemma cancel_to_1_append_left: "cancels_to_1 a b ==> cancels_to_1 (l@a) (l@b)"
-apply(simp add:cancels_to_1_def)
-apply(erule exE)
-apply(rule_tac x="length l + i" in exI)
-apply(auto simp add:cancels_to_1_at_def nth_append cancel_at_def)
-done
+lemma cancel_to_1_append:
+  assumes "cancels_to_1 a b"
+  shows "cancels_to_1 (l@a@l') (l@b@l')"
+proof-
+  from `cancels_to_1 a b` obtain i where "cancels_to_1_at i a b"
+    by -(simp add: cancels_to_1_def, erule exE)
+  hence "cancels_to_1_at (length l + i) (l@a@l') (l@b@l')"
+    by (auto simp add:cancels_to_1_at_def nth_append cancel_at_def)
+  thus "cancels_to_1 (l@a@l') (l@b@l')"
+    by (auto simp add: cancels_to_1_def)
+qed
 
-lemma cancel_to_1_append_right: "cancels_to_1 a b ==> cancels_to_1 (a@l) (b@l)"
-apply(simp add:cancels_to_1_def)
-apply(erule exE)
-apply(rule_tac x="i" in exI)
-apply(auto simp add:cancels_to_1_at_def nth_append cancel_at_def)
-done
+lemma cancel_to_append:
+  assumes "cancels_to a b"
+  shows "cancels_to (l@a@l') (l@b@l')"
+proof-
+  from `cancels_to a b`
+  have "cancels_to_1^** a b" by (simp add:cancels_to_def)
+  thus ?thesis
+  proof(induct rule:rtranclp.induct)
+    fix a
+    show "cancels_to (l @ a @ l') (l @ a @ l')" by (simp add:cancels_to_def)
+  next
+    fix a b c
+    assume "cancels_to (l @ a @ l') (l @ b @ l')"
+    assume "cancels_to_1 b c"
+    hence "cancels_to_1 (l @ b @ l') (l @ c @ l')" by (rule cancel_to_1_append)
+    with `cancels_to (l @ a @ l') (l @ b @ l')`
+    show "cancels_to (l @ a @ l') (l @ c @ l')" by (auto simp add:cancels_to_def)
+  qed
+qed
 
-lemma cancel_to_append_left: "cancels_to a b ==> cancels_to (l@a) (l@b)"
-apply(simp add:cancels_to_def)
-apply(induct rule:rtranclp.induct)
-apply auto
-apply(subgoal_tac "cancels_to_1 (l@b) (l@c)")
-prefer 2
-apply(rule cancel_to_1_append_left)
-apply assumption
-apply auto
-done
-
-lemma cancel_to_append_right: "cancels_to a b ==> cancels_to (a@l) (b@l)"
-apply(simp add:cancels_to_def)
-apply(induct rule:rtranclp.induct)
-apply auto
-apply(subgoal_tac "cancels_to_1 (b@l) (c@l)")
-prefer 2
-apply(rule cancel_to_1_append_right)
-apply assumption
-apply auto
-done
-
-lemma cancel_to_append: "[| cancels_to a a' ; cancels_to b b' |] ==> cancels_to (a@b) (a'@b')"
-apply(subgoal_tac  "cancels_to (a@b) (a@b')")
-prefer 2
-apply(rule cancel_to_append_left)
-apply assumption
-apply(simp add:cancels_to_def)
-apply(induct rule:rtranclp.induct)
-apply auto
-apply(subgoal_tac "cancels_to_1 (ba@b') (c@b')")
-prefer 2
-apply(rule cancel_to_1_append_right)
-apply assumption
-apply auto
-done
+lemma cancels_to_append2:
+  assumes "cancels_to a a'"
+      and "cancels_to b b'"
+  shows "cancels_to (a@b) (a'@b')"
+proof-
+  from `cancels_to a a'`
+  have "cancels_to_1^** a a'" by (simp add:cancels_to_def)
+  thus ?thesis
+  proof(induct rule:rtranclp.induct)
+   fix a
+   from `cancels_to b b'`
+   have "cancels_to (a@b@[]) (a@b'@[])" by (rule cancel_to_append)
+   thus "cancels_to (a@b) (a@b')" by simp
+  next
+   fix a ba c
+   assume "cancels_to_1 (ba :: (bool \<times> 'a) list) c" (* Why do I have to fix the type here? *)
+   hence "cancels_to_1 ([]@ba@b') ([]@c@b')" by (rule cancel_to_1_append)
+   hence "cancels_to_1 (ba@b') (c@b')" by simp
+   moreover
+   assume "cancels_to (a @ b) (ba @ b')"
+   ultimately
+   show "cancels_to (a @ b) (c @ b')" by (simp add:cancels_to_def)
+  qed
+qed
 
 text {*
 The empty list is cancelled.
@@ -343,7 +438,8 @@ The empty list is cancelled.
 lemma empty_canceled[simp]: "canceled []"
 by(auto simp:add canceled_def cancels_to_1_def cancels_to_1_at_def)
 
-lemma cancels_to_self[simp]: "cancels_to l l" by(simp add:cancels_to_def)
+lemma cancels_to_self[simp]: "cancels_to l l"
+by (simp add:cancels_to_def)
 
 subsection {* Definition of normalization *}
 
@@ -353,105 +449,110 @@ Using the THE construct, we can define the normalization function
 to.
 *}
 
-definition normalize :: "'a word_g_i => 'a word_g_i"
+definition normalize :: "'a word_g_i \<Rightarrow> 'a word_g_i"
 where "normalize l = (THE l'. cancels_to l l' \<and> canceled l')"
 
 text {*
 Some obvious properties of the normalize function, and other useful lemmas.
 *}
 
-lemma foo: "\<exists>l'. cancels_to l l' \<and> canceled l'"
-apply(insert canceling_terminates)
-apply(simp add:cancels_to_def canceled_def)
-apply(simp add:wfP_eq_minimal)
-apply(erule_tac x="{l'. cancels_to_1^** l l'}" in allE)
-apply auto
-apply(rule_tac x="z" in exI)
-apply auto
-apply(erule_tac x="b" in allE)
-apply auto
-apply(subgoal_tac "cancels_to_1^** l b")
-apply auto[1]
-apply(subgoal_tac "cancels_to_1^** z b")
-prefer 2
-apply (auto)[1]
-apply(erule rtranclp_trans)
-apply assumption
-done
+lemma
+  shows normalized_canceled[simp]: "canceled (normalize l)"
+  and   normalized_cancels_to[simp]: "cancels_to l (normalize l)"
+proof-
+  thm canceling_terminates
+  let ?Q = "{l'. cancels_to_1^** l l'}"
+  have "l \<in> ?Q" by (auto) hence "\<exists>x. x \<in> ?Q" by (rule exI)
 
-lemma foo': "(!!l'. cancels_to l l' \<and> canceled l' ==> P) ==> P"
-apply(insert foo)
-apply(rotate_tac 1)
-apply(erule_tac x=l in meta_allE)
-apply(rotate_tac 1)
-apply(erule exE)
-apply(erule_tac x=l' in meta_allE)
-apply auto
-done
+  have "wfP cancels_to_1^--1"
+    by (rule canceling_terminates)
+  hence "\<forall>Q. (\<exists>x. x \<in> Q) \<longrightarrow> (\<exists>z\<in>Q. \<forall>y. cancels_to_1 z y \<longrightarrow> y \<notin> Q)"
+    by (simp add:wfP_eq_minimal)
+  hence "(\<exists>x. x \<in> ?Q) \<longrightarrow> (\<exists>z\<in>?Q. \<forall>y. cancels_to_1 z y \<longrightarrow> y \<notin> ?Q)"
+    by (erule_tac x="?Q" in allE)
+  with `\<exists>x. x \<in> ?Q`
+  have "\<exists>z\<in>?Q. \<forall>y. cancels_to_1 z y \<longrightarrow> y \<notin> ?Q" by -(rule mp)
+  then obtain l' where "l' \<in> ?Q" and "(\<forall>y. cancels_to_1 l' y \<longrightarrow> y \<notin> ?Q)" by auto
+  
+  from `l' \<in> ?Q` have "cancels_to l l'" by (auto simp add: cancels_to_def)
 
-lemma normalized_props: "cancels_to l (normalize l) \<and> canceled (normalize l)"
-apply(rule_tac l=l in foo')
-apply (simp add:normalize_def)
-apply(rule_tac a="l'" in theI)
-apply (auto elim:norm_form_uniq)
-done
+  have "canceled l'"
+  proof(rule ccontr)
+    assume "\<not> canceled l'" hence "DomainP cancels_to_1 l'" by (simp add: canceled_def)
+    then obtain y where "cancels_to_1 l' y" by auto
+    with `cancels_to l l'` have "cancels_to l y" by (auto simp add: cancels_to_def)
+    from `\<forall>y. cancels_to_1 l' y \<longrightarrow> y \<notin> ?Q`
+    have "cancels_to_1 l' y \<longrightarrow> y \<notin> ?Q" by auto
+    with `cancels_to_1 l' y` have "y \<notin> ?Q" by -(rule mp)
+    hence "\<not> cancels_to_1^** l y" by auto
+    hence "\<not> cancels_to l y" by (simp add: cancels_to_def)
+    with `cancels_to l y` show False by contradiction
+  qed
 
-lemma normalized_canceled[simp]: "canceled (normalize l)" by (auto simp add:normalized_props)
+  from `cancels_to l l'` and `canceled l'`
+  have "cancels_to l l' \<and> canceled l'" by simp
+  hence "cancels_to l (normalize l) \<and> canceled (normalize l)"
+  proof (simp add:normalize_def, rule theI)
+    fix l'a
+    assume "cancels_to l l' \<and> canceled l'"
+       and "cancels_to l l'a \<and> canceled l'a"
+    thus "l'a = l'" by (auto elim:norm_form_uniq)
+  qed
+  thus "canceled (normalize l)" and "cancels_to l (normalize l)" by auto
+qed
 
-lemma normalized_cancels_to[simp]: "cancels_to l (normalize l)" by (auto simp add:normalized_props)
-
-
-lemma normalize_discover: "[| canceled l'; cancels_to l l' |] ==> normalize l = l'"
-apply(subgoal_tac "cancels_to l l' \<and> canceled l'")
-prefer 2
-apply auto[1]
-apply(simp add:normalize_def)
-apply (auto elim:norm_form_uniq)
-done
+lemma normalize_discover:
+  assumes "canceled l'"
+      and "cancels_to l l'"
+  shows "normalize l = l'"
+proof-
+  from `canceled l'` and `cancels_to l l'`
+  have "cancels_to l l' \<and> canceled l'" by auto
+  thus ?thesis by (auto simp add:normalize_def elim:norm_form_uniq)
+qed
 
 text {* Words, related by cancelation, have the same normal form *}
 
-lemma normalize_canceled[simp]: "cancels_to l l' ==> normalize l = normalize l'"
-apply(rule normalize_discover)
-apply auto
-apply(simp add:normalize_def)
-apply(rule_tac a="normalize l'" in theI2)
-apply auto
-apply(auto simp add:cancels_to_def normalize_discover)
-done
-
+lemma normalize_canceled[simp]:
+  assumes "cancels_to l l'"
+  shows   "normalize l = normalize l'"
+proof(rule normalize_discover)
+  show "canceled (normalize l')" by (rule normalized_canceled)
+next
+  have "cancels_to l' (normalize l')" by (rule normalized_cancels_to)
+  with `cancels_to l l'`
+  show "cancels_to l (normalize l')" by (rule cancels_to_trans)
+qed
 
 text {* Normalization is idempotent *}
 
-lemma normalize_idemp[simp]: "[| canceled l  |] ==> normalize l = l"
-apply(erule  normalize_discover)
-apply(auto simp add:cancels_to_def)
-done
+lemma normalize_idemp[simp]:
+  assumes "canceled l"
+  shows "normalize l = l"
+proof(rule normalize_discover)
+  from `canceled l` show "canceled l".
+next
+  show "cancels_to l l" by (rule cancels_to_self)
+qed
 
 text {*
 This lemma lifts the distributivity results from above to the normalize
 function.
 *}
 
-lemma normalize_append_cancel_to: "[| cancels_to l1 l1' ; cancels_to l2 l2'  |] ==> normalize (l1 @ l2) = normalize (l1' @ l2')"
-apply(subgoal_tac "cancels_to (l1 @ l2) (normalize (l1@l2))")
-prefer 2
-apply(auto simp add: normalized_props)[1]
-
-apply(subgoal_tac "cancels_to (l1 @ l2) (normalize (l1'@l2'))")
-prefer 2
-
-apply(subgoal_tac "cancels_to (l1 @ l2) (l1'@l2')")
-prefer 2
-apply(rule cancel_to_append)
-apply assumption+
-
-apply(subgoal_tac "cancels_to (l1' @ l2') (normalize (l1'@l2'))")
-prefer 2
-apply(auto simp add: normalized_props)[1]
-
-apply(simp only:cancels_to_def)
-apply auto[1]
-done
+lemma normalize_append_cancel_to:
+  assumes "cancels_to l1 l1'"
+  and     "cancels_to l2 l2'"
+  shows "normalize (l1 @ l2) = normalize (l1' @ l2')"
+proof(rule normalize_discover)
+  show "canceled (normalize (l1' @ l2'))" by (rule normalized_canceled)
+next
+  from `cancels_to l1 l1'` and `cancels_to l2 l2'`
+  have "cancels_to (l1 @ l2) (l1' @ l2')" by (rule cancels_to_append2)
+  moreover
+  have "cancels_to (l1' @ l2') (normalize (l1' @ l2'))" by (rule normalized_cancels_to)
+  ultimately
+  show "cancels_to (l1 @ l2) (normalize (l1' @ l2'))"  by (rule cancels_to_trans)
+qed
 
 end
