Free-Groups.thy
@@ -7,12 +7,20 @@ begin
 text {*
 Based on the work in @{theory Cancelation}, the free group is now easily defined
 over the set of fully canceled words.
+
+Because the definition of the set is so short, we want it to be unrolled by the
+simplifier.
 *}
 
-typedef 'a free_group_set = "{x :: 'a word_g_i. canceled x}"
-apply(rule_tac x="[]" in exI)
-apply (auto simp add:normalize_def)
-done
+typedef 'a free_group_set = "{x :: 'a word_g_i. canceled x}" 
+proof-
+  have "canceled []" by simp
+  thus ?thesis by blast
+qed
+
+lemma free_group_set_simp[simp]:
+"l \<in> free_group_set = canceled l"
+by (simp add: free_group_set_def)
 
 text {*
 Multiplication is concatenation, followed by normalization.
@@ -29,9 +37,8 @@ a single generator, and show that it is self-inverse.
 definition inv1 :: "'a g_i \<Rightarrow> 'a g_i"
  where "inv1 a = (\<not> fst a, snd a)"
 
-lemma inv1_inv1[simp]: "inv1 \<circ> inv1 = id"
-apply(simp add: expand_fun_eq comp_def inv1_def)
-done
+lemma inv1_inv1[simp]: "inv1 \<circ> inv1 = (\<lambda>x. x)"
+  by (simp add: expand_fun_eq comp_def inv1_def)
 
 text {*
 The inverse of a word is obtained by reversing the order of the generator and
@@ -43,30 +50,94 @@ definition inv_fg :: "'a word_g_i \<Rightarrow> 'a word_g_i"
  where "inv_fg l = rev (map inv1 l)"
 
 lemma cancelling_inf[simp]: "canceling (inv1 a) (inv1 b) = canceling a b"
-apply(simp add: canceling_def inv1_def)
-done
+  by(simp add: canceling_def inv1_def)
 
-lemma inv_fg_closure: "l \<in> free_group_set \<Longrightarrow> inv_fg l \<in> free_group_set"
-apply(simp add:inv_fg_def free_group_set_def canceled_def)
-apply(auto)
-apply(subgoal_tac "cancels_to_1 l (rev (map inv1 b))")
-apply auto[1]
-apply(thin_tac "\<not> DomainP cancels_to_1 l")
+lemma inv_idemp: "inv_fg (inv_fg l) = l"
+  by (auto simp add:inv_fg_def rev_map)
 
+lemma inv_fg_cancel: "mult_norm l (inv_fg l) = []"
+proof(induct l rule:rev_induct)
+  show "mult_norm [] (inv_fg []) = []"
+    by (auto simp add:mult_norm_def inv_fg_def)
+next
+  fix x :: "'a g_i"
+  fix xs :: "'a word_g_i"
+  assume "mult_norm xs (inv_fg xs) = []"
+  hence "normalize (xs @ (inv_fg xs)) = []" by (auto simp add:mult_norm_def)
 
-apply(simp add:cancels_to_1_def)
-apply auto[1]
+  have "canceling x (inv1 x)" by (simp add:inv1_def canceling_def)
+  moreover
+  let ?i = "length xs"
+  have "Suc ?i < length xs + 1 + 1 + length xs"
+    by auto
+  moreover
+  have "inv_fg (xs @ [x]) = [inv1 x] @ inv_fg xs"
+    by (auto simp add:inv_fg_def)
+  ultimately
+  have "cancels_to_1_at ?i (xs @ [x] @ (inv_fg (xs @ [x]))) (xs @ inv_fg xs)"
+    by (auto simp add:cancels_to_1_at_def cancel_at_def nth_append)
+  hence "cancels_to_1 (xs @ [x] @ (inv_fg (xs @ [x]))) (xs @ inv_fg xs)"
+    by (auto simp add: cancels_to_1_def)
+  hence "cancels_to (xs @ [x] @ (inv_fg (xs @ [x]))) (xs @ inv_fg xs)"
+    by (auto simp add:cancels_to_def)
+  with `normalize (xs @ (inv_fg xs)) = []`
+  have "normalize (xs @ [x] @ (inv_fg (xs @ [x]))) = []"
+    by auto
+  thus "mult_norm (xs @ [x]) (inv_fg (xs @ [x])) = []"
+    by (auto simp add:mult_norm_def)
+qed
 
-apply(rule_tac x="length l - i - 2" in exI)
-apply(auto simp add:cancels_to_1_at_def)
-apply(auto simp add:rev_nth)
-apply(rule cancel_sym)
-apply(subgoal_tac "Suc (length l - Suc (Suc i)) = length l - Suc i")
-apply simp
-apply auto[1]
-apply(subgoal_tac "Suc (Suc (length l - Suc (Suc i))) = length l - i")
-apply(auto simp add: id_def cancel_at_def rev_map rev_take rev_drop take_map drop_map)
-done
+lemma inv_fg_cancel2: "mult_norm (inv_fg l) l = []"
+proof-
+  have "mult_norm (inv_fg l) (inv_fg (inv_fg l)) = []" by (rule inv_fg_cancel)
+  thus "mult_norm (inv_fg l) l = []" by (simp add: inv_idemp)
+qed
+
+lemma inv_fg_closure:
+  assumes "l \<in> free_group_set"
+  shows "inv_fg l \<in> free_group_set"
+proof-
+  from `l \<in> free_group_set` have "canceled l" by simp
+  have "canceled (inv_fg l)"
+  proof(rule ccontr)
+    assume "\<not>canceled (inv_fg l)"
+    hence "DomainP cancels_to_1 (inv_fg l)" by (simp add: canceled_def)
+    then obtain l' where "cancels_to_1 (inv_fg l) l'" by auto
+    then obtain i where "cancels_to_1_at i (inv_fg l) l'" by (auto simp add:cancels_to_1_def)
+    hence "Suc i < length (inv_fg l)"
+      and "canceling (inv_fg l ! i) (inv_fg l ! Suc i)"
+      by (auto simp add:cancels_to_1_at_def)
+    let ?x = "length l - i - 2"
+    from `Suc i < length (inv_fg l)`
+    have "Suc i < length l" by (simp add: inv_fg_def)
+    hence "Suc ?x < length l" by auto
+
+    moreover
+    from `Suc i < length l`
+    have "i < length l" and "length l - Suc i = Suc(length l - Suc (Suc i))" by auto
+    hence "inv_fg l ! i = inv1 (l ! Suc ?x)"
+      by (auto simp add:inv_fg_def rev_nth map_nth)
+    from `Suc i < length l`
+    have "inv_fg l ! Suc i = inv1 (l ! ?x)"
+      by (auto simp add:inv_fg_def rev_nth map_nth)
+    from `canceling (inv_fg l ! i) (inv_fg l ! Suc i)`
+     and `inv_fg l ! i = inv1 (l ! Suc ?x)`
+     and `inv_fg l ! Suc i = inv1 (l ! ?x)`
+    have "canceling (inv1 (l ! Suc ?x)) (inv1 (l ! ?x))" by auto
+    hence "canceling (inv1 (l ! ?x)) (inv1 (l ! Suc ?x))" by (rule cancel_sym)
+    hence "canceling (l ! ?x) (l ! Suc ?x)" by simp
+
+    ultimately
+    have "cancels_to_1_at ?x l (cancel_at ?x l)" 
+      by (auto simp add:cancels_to_1_at_def)
+    hence "cancels_to_1 l (cancel_at ?x l)"
+      by (auto simp add:cancels_to_1_def)
+    hence "\<not>canceled l"
+      by (auto simp add:canceled_def)
+    with `canceled l` show False by contradiction
+  qed
+  thus "inv_fg l \<in> free_group_set" by simp
+qed
 
 text {*
 Finally, we can define the Free Group, and show that it is indeed a group.
@@ -76,47 +147,62 @@ constdefs
   "free_group \<equiv> (|carrier = free_group_set, mult = mult_norm, one = []|)"
 
 lemma  "group free_group"
-unfolding free_group_def
-apply(rule groupI)
-apply(auto)
-apply(simp add:mult_norm_def free_group_set_def)
-apply(simp add:empty_canceled free_group_set_def)
-prefer 2
-apply(auto elim: normalize_idemp simp add:mult_norm_def free_group_set_def)[1]
-
-apply(simp add:mult_norm_def)
-apply(subgoal_tac "normalize (normalize (x @ y) @ z) = normalize ((x @ y) @ z)")
-prefer 2
-apply(rule sym)
-apply(rule normalize_append_cancel_to)
-apply auto
-apply(subgoal_tac "normalize (x @ normalize (y @ z)) = normalize (x @ (y @ z))")
-prefer 2
-apply(rule sym)
-apply(rule normalize_append_cancel_to)
-apply auto
-
-apply(rename_tac l)
-apply(rule_tac x="inv_fg l" in bexI)
-apply(induct_tac l)
-apply(auto simp add:inv_fg_def mult_norm_def)[1]
-apply(auto simp add:inv_fg_def mult_norm_def)[1]
-apply(subgoal_tac "cancels_to (rev (map inv1 list) @ inv1 (a, b) # (a, b) # list)  (rev (map inv1 list) @ list)")
-apply auto[1]
-apply(subgoal_tac "cancels_to (inv1 (a, b) # (a, b) # list) list")
-prefer 2
-apply(subgoal_tac "cancels_to_1_at 0 (inv1 (a, b) # (a, b) # list) list")
-prefer 2
-apply(simp add:cancels_to_1_at_def inv1_def cancel_at_def canceling_def)
-apply(simp add:cancels_to_def)
-apply(rule  r_into_rtranclp )
-apply(simp add:cancels_to_1_def)
-apply(rule_tac x="0" in exI)
-apply assumption
-apply(rule cancel_to_append_left)
-apply assumption
-apply(rule inv_fg_closure)
-apply assumption
-done
+proof
+  fix x y
+  show "x \<otimes>\<^bsub>free_group\<^esub> y \<in> carrier free_group"
+    by (auto simp add:mult_norm_def free_group_def)
+next
+  fix x y z
+  have "cancels_to (x @ y) (normalize (x @ (y::'a word_g_i)))"
+   and "cancels_to z (z::'a word_g_i)"
+    by auto
+  hence "normalize (normalize (x @ y) @ z) = normalize ((x @ y) @ z)"
+    by (rule normalize_append_cancel_to[THEN sym])
+  moreover
+  have "\<dots> = normalize (x @ (y @ z))" by auto
+  moreover
+  have "cancels_to (y @ z) (normalize (y @ (z::'a word_g_i)))"
+   and "cancels_to x (x::'a word_g_i)"
+    by auto
+  hence "normalize (x @ (y @ z)) = normalize (x @ normalize (y @ z))"
+    by -(rule normalize_append_cancel_to)
+  ultimately
+  have "normalize (normalize (x @ y) @ z) = normalize (x @ normalize (y @ z))"
+    by simp
+  thus "x \<otimes>\<^bsub>free_group\<^esub> y \<otimes>\<^bsub>free_group\<^esub> z =
+        x \<otimes>\<^bsub>free_group\<^esub> (y \<otimes>\<^bsub>free_group\<^esub> z)"
+    by (auto simp add:mult_norm_def free_group_def)
+next
+  show "\<one>\<^bsub>free_group\<^esub> \<in> carrier free_group" 
+    by (auto simp add:free_group_def)
+next
+  fix x
+  assume "x \<in> carrier free_group" 
+  thus "\<one>\<^bsub>free_group\<^esub> \<otimes>\<^bsub>free_group\<^esub> x = x"
+    by (auto simp add:free_group_def mult_norm_def)
+next
+  fix x
+assume "x \<in> carrier free_group"
+  thus "x \<otimes>\<^bsub>free_group\<^esub> \<one>\<^bsub>free_group\<^esub> = x"
+    by (auto simp add:free_group_def mult_norm_def)
+next
+  show "carrier free_group \<subseteq> Units free_group"
+  proof (simp add:free_group_def Units_def, rule subsetI)
+    fix x :: "'b word_g_i"
+    let ?x = "inv_fg x"
+    assume "x \<in> free_group_set"
+    hence "?x \<in> free_group_set" by (rule inv_fg_closure)
+    moreover
+    have "mult_norm ?x x = []"
+     and "mult_norm x ?x = []"
+      by (auto simp add: inv_fg_cancel inv_fg_cancel2)
+    ultimately
+    have "\<exists>x'\<in>free_group_set. mult_norm x' x = [] \<and> mult_norm x x' = []" by auto
+    with `x \<in> free_group_set`
+    show "x \<in> {y. canceled y \<and>
+               (\<exists>x \<in>free_group_set. mult_norm x y = [] \<and> mult_norm y x = [])}"
+      by auto
+   qed
+qed
 
 end
